cleaning stuff and addings comments

theories/refinements/static_gradual/compat_cast/defs.v
@@ -1,33 +1,10 @@
-From fae_gtlc_mu.refinements.static_gradual Require Export logical_relation resources_right compat_easy.
-From fae_gtlc_mu.cast_calculus Require Export types typing.
-From fae_gtlc_mu.stlc_mu Require Export lang.
+From fae_gtlc_mu.refinements.static_gradual Require Export logical_relation.
+From fae_gtlc_mu.backtranslation Require Export alternative_consistency.
+From fae_gtlc_mu.backtranslation Require Export cast_help.general_def.
 From fae_gtlc_mu.cast_calculus Require Export lang.
-From iris.algebra Require Import list.
-From iris.proofmode Require Import tactics.
-From iris.program_logic Require Import lifting.
-From fae_gtlc_mu.cast_calculus Require Export types.
-From fae_gtlc_mu.cast_calculus Require Export consistency.
-From fae_gtlc_mu.backtranslation Require Export cast_help.general_def cast_help.extract cast_help.embed.
-From fae_gtlc_mu.cast_calculus Require Export lang.
-
-(* Coercion stlc_mu.lang.of_val : stlc_mu.lang.val >-> stlc_mu.lang.expr. *)
-(* Coercion cast_calculus.lang.of_val : cast_calculus.lang.val >-> cast_calculus.lang.expr. *)
-
-(* Notation "# v" := (of_val v) (at level 20). *)
 
 Section defs.
   Context `{!implG Σ,!specG Σ}.
-  Notation D := (prodO stlc_mu.lang.valO cast_calculus.lang.valO -n> iPropO Σ).
-  (* Implicit Types e : stlc_mu.lang.expr. *)
-  (* Implicit Types e : stlc_mu.lang.expr. *)
-  Implicit Types fs : list stlc_mu.lang.val.
-  (* Implicit Types f : stlc_mu.lang.val. *)
-  Implicit Types A : list (cast_calculus.types.type * cast_calculus.types.type).
-  (* Implicit Types a : (cast_calculus.types.type * cast_calculus.types.type). *)
-  Local Hint Resolve to_of_val : core.
-
-  (** We will want to assume these functions to be meaningful..,
-      i.e. they properly relate to the casts happening on the right side *)
 
   Definition rel_cast_functions A (fs : list stlc_mu.lang.val) : iProp Σ :=
     ⌜length A = length fs⌝ ∗
@@ -47,9 +24,8 @@ Section defs.
   (** The statement that the -- closed up -- back-translated casts behave appropriately.
       (We redefine it here to a new statement, making it a bit more amenable for proving.) *)
 
-  (* TODO!! 𝓕cV instead of 𝓕c *)
-
   Definition back_cast_ar {A} {τi τf} (pC : alternative_consistency A τi τf) :=
   ∀ ei' K' v v' fs, (rel_cast_functions A fs ∧ ⟦ τi ⟧ (v, v') ∧ initially_inv ei' ∧ currently_half (fill K' (Cast (cast_calculus.lang.of_val v') τi τf)))
-                     ⊢ (WP (𝓕c pC fs (stlc_mu.lang.of_val v)) {{ w, ∃ w', currently_half (fill K' (cast_calculus.lang.of_val w')) ∧ ⟦ τf ⟧ (w, w') }})%I.
+                     ⊢ (WP 𝓕c pC fs (stlc_mu.lang.of_val v) {{ w, ∃ w', currently_half (fill K' (cast_calculus.lang.of_val w')) ∧ ⟦ τf ⟧ (w, w') }})%I.
+
 End defs.
