theories/refinements/gradual_static/compat_cast/all.v
@@ -1,37 +1,13 @@
-From fae_gtlc_mu.stlc_mu Require Export types typing.
-From fae_gtlc_mu.cast_calculus Require Export lang.
-From iris.algebra Require Import list.
-From iris.proofmode Require Import tactics.
-From iris.program_logic Require Import lifting.
-From fae_gtlc_mu.backtranslation Require Export cast_help.general_def cast_help.extract cast_help.embed.
-From fae_gtlc_mu.stlc_mu Require Export lang.
-From fae_gtlc_mu.refinements.gradual_static Require Export logical_relation resources_left resources_right compat_easy compat_cast.defs.
-From fae_gtlc_mu.cast_calculus Require Export types.
-From fae_gtlc_mu.refinements.gradual_static.compat_cast Require Export between_rec prod_prod sum_sum arrow_arrow identity tau_star ground_star tau_star star_tau star_ground.
+From fae_gtlc_mu.refinements.gradual_static Require Export logical_relation compat_cast.defs compat_easy.
+From fae_gtlc_mu.refinements.gradual_static.compat_cast Require Export
+     between_rec prod_prod sum_sum arrow_arrow identity tau_star ground_star tau_star star_tau star_ground.
 
 Section compat_cast_all.
   Context `{!implG Σ,!specG Σ}.
-  Notation D := (prodO cast_calculus.lang.valO stlc_mu.lang.valO -n> iPropO Σ).
-  Implicit Types fs : list stlc_mu.lang.val.
-  (* Implicit Types f : stlc_mu.lang.val. *)
-  Implicit Types A : list (cast_calculus.types.type * cast_calculus.types.type).
-  Local Hint Resolve to_of_val : core.
-  Local Hint Resolve cast_calculus.lang.to_of_val : core.
 
   Lemma back_cast_ar_all {A} {τi τf} (pC : alternative_consistency A τi τf) : back_cast_ar pC.
   Proof.
-    induction pC.
-    - by apply back_cast_ar_star_ground.
-    - by apply back_cast_ar_ground_star.
-    - by apply back_cast_ar_tau_star.
-    - by apply back_cast_ar_star_tau.
-    - by apply back_cast_ar_base_base.
-    - by apply back_cast_ar_star_star.
-    - by apply back_cast_ar_sum_sum.
-    - by apply back_cast_ar_prod_prod.
-    - by apply back_cast_ar_arrow_arrow.
-    - by apply back_cast_ar_trec_trec_expose.
-    - by apply back_cast_ar_trec_trec_use.
+    induction pC; eauto using back_cast_ar_star_ground, back_cast_ar_ground_star, back_cast_ar_tau_star, back_cast_ar_star_tau, back_cast_ar_base_base, back_cast_ar_star_star, back_cast_ar_sum_sum, back_cast_ar_prod_prod, back_cast_ar_arrow_arrow, back_cast_ar_trec_trec_expose, back_cast_ar_trec_trec_use.
   Qed.
 
   Notation "'` H" := (bin_log_related_alt H) (at level 8).
