theories/refinements/gradual_static/compat_cast/ground_star.v
@@ -1,35 +1,12 @@
-From fae_gtlc_mu.stlc_mu Require Export types typing.
-From fae_gtlc_mu.cast_calculus Require Export lang.
-From iris.algebra Require Import list.
-From iris.proofmode Require Import tactics.
-From iris.program_logic Require Import lifting.
-From fae_gtlc_mu.backtranslation Require Export cast_help.general_def cast_help.extract cast_help.embed props.extract_embed.
+From fae_gtlc_mu.refinements.gradual_static Require Export compat_cast.defs.
+From fae_gtlc_mu.backtranslation Require Export general_def_lemmas.
 From fae_gtlc_mu.stlc_mu Require Export lang.
-From fae_gtlc_mu.refinements.gradual_static Require Export logical_relation resources_left resources_right compat_easy compat_cast.defs.
 From fae_gtlc_mu.cast_calculus Require Export types.
 
 Section ground_star.
   Context `{!implG Σ,!specG Σ}.
-  Notation D := (prodO cast_calculus.lang.valO stlc_mu.lang.valO -n> iPropO Σ).
-  (* Implicit Types e : cast_calculus.lang.expr. *)
-  (* Implicit Types e : cast_calculus.lang.expr. *)
-  Implicit Types fs : list cast_calculus.lang.val.
-  (* Implicit Types f : cast_calculus.lang.val. *)
-  Implicit Types A : list (stlc_mu.types.type * stlc_mu.types.type).
-  (* Implicit Types a : (stlc_mu.types.type * stlc_mu.types.type). *)
-  Local Hint Resolve to_of_val : core.
-  Local Hint Resolve cast_calculus.lang.to_of_val : core.
-
-  Hint Resolve to_of_val : core.
 
   Hint Extern 5 (AsVal _) => eexists; simpl; try done; eapply cast_calculus.lang.of_to_val; fast_done : typeclass_instances.
-  Hint Extern 10 (AsVal _) =>
-  eexists; rewrite /IntoVal; eapply of_to_val; rewrite /= !to_of_val /=; solve [ eauto ] : typeclass_instances.
-
-
-  Hint Extern 5 (IntoVal _ _) => eapply of_to_val; fast_done : typeclass_instances.
-  Hint Extern 10 (IntoVal _ _) =>
-    rewrite /IntoVal; eapply of_to_val; rewrite /= !to_of_val /=; solve [ eauto ] : typeclass_instances.
 
   Lemma back_cast_ar_ground_star:
     ∀ (A : list (type * type)) (τG : type) (G : Ground τG), back_cast_ar (atomic_Ground_Unknown A τG G).
@@ -67,10 +44,9 @@ Section ground_star.
       iMod ((step_Fold _ ei' (InjRCtx :: FoldCtx :: K')) with "[Hv']") as "Hv'"; auto.
       iApply (wp_value _ _ _ _ (CastV (cast_calculus.lang.FoldV u) (TRec ⋆) ⋆ (TGround_TUnknown_icp (Ground_TRec)))); try by simpl.
       iExists (embedV_TUnknown u'). iFrame "Hv'".
-      rewrite (interp_rw_TUnknown (CastV (lang.FoldV u) (TRec ⋆) ⋆ (TGround_TUnknown_icp Ground_TRec), embedV_TUnknown u')).
+      rewrite (interp_rw_TUnknown (CastV (cast_calculus.lang.FoldV u) (TRec ⋆) ⋆ (TGround_TUnknown_icp Ground_TRec), embedV_TUnknown u')).
       iExists _ , _.
       iModIntro. iRight. iRight. iRight. iRight. iSplit; done.
   Qed.
-
 
 End ground_star.
