theories/refinements/static_gradual/compat_cast/between_rec.v
@@ -1,23 +1,9 @@
-From fae_gtlc_mu.refinements.static_gradual Require Export logical_relation resources_right compat_easy compat_cast.defs.
-From fae_gtlc_mu.cast_calculus Require Export types typing.
+From fae_gtlc_mu.refinements.static_gradual Require Export compat_cast.defs.
+From fae_gtlc_mu.backtranslation.cast_help Require Export between_rec_fix.
 From fae_gtlc_mu.cast_calculus Require Export lang.
-From iris.algebra Require Import list.
-From iris.proofmode Require Import tactics.
-From iris.program_logic Require Import lifting.
-From fae_gtlc_mu.backtranslation.cast_help Require Export general_def general_def_lemmas extract embed between_rec_fix.
-From fae_gtlc_mu.cast_calculus Require Export lang types.
 
 Section between_rec.
   Context `{!implG Σ,!specG Σ}.
-  Notation D := (prodO stlc_mu.lang.valO cast_calculus.lang.valO -n> iPropO Σ).
-  (* Implicit Types e : stlc_mu.lang.expr. *)
-  Implicit Types fs : list stlc_mu.lang.val.
-  (* Implicit Types f : stlc_mu.lang.val. *)
-  Implicit Types A : list (cast_calculus.types.type * cast_calculus.types.type).
-  (* Implicit Types a : (cast_calculus.types.type * cast_calculus.types.type). *)
-  Local Hint Resolve to_of_val : core.
-
-  (** Proving it *)
 
   Lemma back_cast_ar_trec_trec_use:
     ∀ (A : list (type * type)) (τl τr : {bind type}) (i : nat) (pμτlμtrinA : A !! i = Some (TRec τl, TRec τr)),
@@ -26,7 +12,6 @@ Section between_rec.
     intros A τl τr i pμτlμtr.
     rewrite /𝓕c /𝓕 /back_cast_ar; iIntros (ei' K' v v' fs) "(#Hfs & #Hvv' & #Hei' & Hv')".
     rewrite /𝓕c /𝓕. asimpl.
-    (** getting the information about the length of the list *)
     iDestruct "Hfs" as "[% Hfs']".
     destruct (fs !! i) as [f | abs] eqn:Hf.
     rewrite (stlc_mu.typing_lemmas.env_subst_lookup _ i f); try done.
@@ -34,7 +19,7 @@ Section between_rec.
       iDestruct (big_sepL2_lookup with "Hfs'") as "#Hf". exact pμτlμtr. exact Hf.
       iApply ("Hf" $! v v' with "Hvv'"). done.
     }
-    { (* trivially impossible case *)
+    {
       assert (Hi : i < length fs). rewrite -H. by eapply lookup_lt_Some.
       assert (Hi' : i >= length fs). by apply lookup_ge_None_1. exfalso. lia.
     }
@@ -49,12 +34,9 @@ Section between_rec.
     rewrite /𝓕c /𝓕 /back_cast_ar; iIntros (ei' K' v v' fs) "(#Hfs & #Hvv' & #Hei' & Hv')".
     (** setting up iLöb *)
     iLöb as "IHlob" forall (v v' ei' K') "Hvv' Hei'".
-    (* fold (𝓕c (exposeRecursiveCAll A τl τr pμτlμτrnotA pC) fs). *)
-    (* iRevert (ei' K' v v') "Hvv' Hei' Hv'". *)
     rewrite {2}/𝓕c. rewrite /𝓕.
     fold (𝓕 pC).
     (** rewriting value relation for v and v' *)
-    (* rewrite fixpoint_interp_rec1_eq. *)
     rewrite interp_rw_TRec.
     iDestruct "Hvv'" as (w w') "#[% Hww']".
     inversion H; clear v v' H H1 H2.
@@ -74,7 +56,6 @@ Section between_rec.
     iApply (wp_wand with "[-]").
     iApply (IHpC ei' (FoldCtx :: K') w w' (𝓕cV (exposeRecursiveCAll A τl τr pμτlμτrnotA pC) fs H :: fs)). iSplitL "Hfs". iSplitR. simpl. by rewrite H.
     (** applying IHlob and Hfs *)
-    (* rewrite /𝓕c. *)
     iSplit.
     iModIntro. iIntros (v v') "#Hvv'".
     { clear K'. iIntros (K') "Hv'". iSimpl in "Hv'".
